riscv aspec+ainvs+haskell: update kernelBase, paddrLoad to match C
update for changeset 897aaf5b13f39ba2b9ca8ade3a58d1350eb42ad7

This changes properties of kernel_base, thereby invalidating two unused
lemmas: mask_out_8_le_kernel_base, mask_out_8_less_kernel_base

spec/abstract/RISCV64/Machine_A.thy
@@ -126,7 +126,7 @@ text \<open>
 \<close>
 definition kernel_base :: "vspace_ref"
   where
-  "kernel_base \<equiv> 0xFFFFFFFF80000000" \<comment> \<open>for Spike platform\<close>
+  "kernel_base \<equiv> 0xFFFFFFFF84000000" \<comment> \<open>for Spike platform\<close>
 
 definition idle_thread_ptr :: vspace_ref
   where
